

Chapter 3 - Linear Regression

1. This is the result of regressing *sales* onto *TV*, *radio* and *newspaper*. From the table we can conclude the following:
 - (a) For a 1000 unit increase in *TV* based ads, keeping *radio* and *newspaper* based ads unchanged, we will observe a 46 unit increase in *sales*.
 - (b) For a 1000 unit increase in *radio* based ads, keeping *TV* and *newspaper* based ads unchanged, we will observe a 189 unit increase in *sales*.
 - (c) We also see that the t-statistic of the coefficient for *newspaper* is very small. Consequently the p-value is close to 1, thus suggesting that *newspaper* is statistically insignificant.
2. For an input x the KNN-classifier will find the K closest points to x and assign the most frequently occurring class amongst the set of close points to x . The KNN-regressor on the other hand will assign the average of the K closest points as the predicted value.
3. X_1 is GPA, X_2 is IQ, X_3 is Gender (1 for Female and 0 for Male), X_4 is the interaction between GPA and IQ, and X_5 is the interaction between GPA and Gender. Thus salary (S) can be equated as follows:

$$S = 50 + 20X_1 + 0.07X_2 + 35X_3 + 0.01X_1X_2 - 10X_1X_3$$

- (a) $S_F = 50 + 20X_1 + 0.07X_2 + 35 + 0.01X_1X_2 - 10X_1$
 $S_M = 50 + 20X_1 + 0.07X_2 + 0.01X_1X_2$

$$S_F - S_M = 35 - 10X_1$$

Now if $35 > 10X_1$ then $S_F > S_M$ else $S_F \leq S_M$. Thus for a given IQ and GPA, males earn more than females provided GPA is high enough.

- (b) $S_F = 50 + 20(4) + 0.07(110) + 35 + 0.01(4)(110) - 10(4)$
 $S_F = 137.1$ units.

- (c) The significance of a predictor cannot be accurately determined from its coefficient (β). The p-value for the t-statistic needs to be computed. The t-statistic is got by dividing β by the standard error of β ($SE(\beta)$). So if $SE(\beta) \ll \beta$ then β will be significant.
4. (a) When comparing based on training RSS, the cubic fit is expected to be slightly better or very similar to the linear fit.
- (b) When comparing based on test RSS, the cubic fit is expected to be worse than the linear fit due to overfitting.
- (c) When comparing based on training RSS, the cubic fit will be much better than the linear fit as the true relationship between the predictors and response is non-linear.
- (d) When comparing based on test RSS, we have two situations that might arise. In the first case if the true relationship is closer to linear than non-linear then the linear fit is expected to do better. If the true relationship is very far from linear, then the cubic fit is expected to have a better test RSS.

5. $\hat{y}_i = x_i \hat{\beta}$ where $\hat{\beta} = \frac{\sum_{i=1}^n x_i y_i}{\sum_{j=1}^n x_j^2}$

$$\hat{y}_i = x_i \frac{\sum_{k=1}^n x_k y_k}{\sum_{j=1}^n x_j^2}$$

$$\hat{y}_i = \frac{x_i x_1 y_1 + x_i x_2 y_2 + \dots x_i x_n y_n}{\sum_{j=1}^n x_j^2}$$

$$\hat{y}_i = \frac{x_i x_1 y_1}{\sum_{j=1}^n x_j^2} + \frac{x_i x_2 y_2}{\sum_{j=1}^n x_j^2} + \dots \frac{x_i x_n y_n}{\sum_{j=1}^n x_j^2}$$

$$\hat{y}_i = \sum_{k=1}^n \frac{x_i x_k}{\sum_{j=1}^n x_j^2} y_k$$

Therefore, $a_k = \frac{x_i x_k}{\sum_{j=1}^n x_j^2}$

6. $Y = \beta_0 + \beta_1 X$

$$\beta_0 = \bar{y} - \beta_1 \bar{x} \text{ and } \beta_1 = \frac{\sum_{i=1}^n (x_i - \bar{x})(y_i - \bar{y})}{\sum_{j=1}^n (x_j - \bar{x})^2}$$

$$Y = \bar{y} - \frac{\sum_{i=1}^n (x_i - \bar{x})(y_i - \bar{y})}{\sum_{j=1}^n (x_j - \bar{x})^2} \bar{x} + \frac{\sum_{i=1}^n (x_i - \bar{x})(y_i - \bar{y})}{\sum_{j=1}^n (x_j - \bar{x})^2} X$$

Now if a line passes through (\bar{x}, \bar{y}) , then for $X = \bar{x}$, Y will be equal to \bar{y} . Plugging $X = \bar{x}$ in the above equation we see that the second and third terms of the equation cancel each other and we are left with $Y = \bar{y}$.

7. $Cor(x, y) = \frac{\sum_{i=1}^n (x_i - \bar{x})(y_i - \bar{y})}{\sqrt{\sum_{j=1}^n (x_j - \bar{x})^2} \sqrt{\sum_{j=1}^n (y_j - \bar{y})^2}}$

Given $\bar{x} = \bar{y} = 0$, $Cor(x, y) = \frac{\sum_{i=1}^n x_i y_i}{\sqrt{\sum_{j=1}^n x_j^2} \sqrt{\sum_{j=1}^n y_j^2}}$

$$R^2 = \frac{TSS - RSS}{TSS} = \frac{\sum_{i=1}^n (y_i - \bar{y})^2 - \sum_{k=1}^n (\hat{y}_k - y_k)^2}{\sum_{j=1}^n (y_j - \bar{y})^2}$$

$$R^2 = \frac{\sum_{i=1}^n y_i^2 - \sum_{i=k}^n (\hat{y}_k - y_k)^2}{\sum_{j=1}^n y_j^2}$$

$$R^2 = 1 - \frac{\sum_{i=k}^n (\hat{y}_k - y_k)^2}{\sum_{j=1}^n y_j^2}$$

Now, $\hat{y}_k = \beta_0 + \beta_1 x_k$. Now since $\bar{x} = \bar{y} = 0$, $\beta_0 = 0$ and $\beta_1 = \frac{\sum_{i=1}^n x_i y_i}{\sum_{j=1}^n x_j^2}$.

$$\sum_{k=1}^n (\hat{y}_k - y_k)^2 = \sum_{k=1}^n (\beta_1 x_k - y_k)^2$$

$$\sum_{k=1}^n (\hat{y}_k - y_k)^2 = \beta_1^2 \sum_{k=1}^n x_k^2 + \sum_{k=1}^n y_k^2 - 2\beta_1 \sum_{k=1}^n x_k y_k$$

$$\frac{\sum_{k=1}^n (\hat{y}_k - y_k)^2}{\sum_{j=1}^n y_j^2} = \beta_1^2 \frac{\sum_{k=1}^n x_k^2}{\sum_{j=1}^n y_j^2} + 1 - 2\beta_1 \frac{\sum_{k=1}^n x_k y_k}{\sum_{j=1}^n y_j^2}$$

$$R^2 = 1 - \frac{\sum_{i=k}^n (\hat{y}_k - y_k)^2}{\sum_{j=1}^n y_j^2} = 2\beta_1 \frac{\sum_{k=1}^n x_k y_k}{\sum_{j=1}^n y_j^2} - \beta_1^2 \frac{\sum_{k=1}^n x_k^2}{\sum_{j=1}^n y_j^2}$$

Substituting $\beta_1 = \frac{\sum_{i=1}^n x_i y_i}{\sum_{j=1}^n x_j^2}$ in the above equation we get,

$$R^2 = 2 \frac{\sum_{i=1}^n x_i y_i}{\sum_{j=1}^n x_j^2} \frac{\sum_{k=1}^n x_k y_k}{\sum_{j=1}^n y_j^2} - \frac{(\sum_{i=1}^n x_i y_i)^2}{(\sum_{j=1}^n x_j^2)^2} \frac{\sum_{k=1}^n x_k^2}{\sum_{j=1}^n y_j^2}$$

$$\text{Thus, } R^2 = \frac{(\sum_{i=1}^n x_i y_i)^2}{\sum_{j=1}^n x_j^2 \sum_{j=1}^n y_j^2} = \text{Cor}(x, y)^2.$$